Fix SequenceFormat against new specs definition.

src/Narcissus/Formats/Base/SequenceFormat.v
@@ -1,8 +1,7 @@
 Require Import
         Fiat.Computation
         Fiat.Common.DecideableEnsembles
-        Fiat.Narcissus.Common.Specs
-        Fiat.Narcissus.Common.ComposeOpt
+        Fiat.Narcissus.Common.SpecsSimpl
         Fiat.Narcissus.Common.Notations
         Fiat.Narcissus.Formats.Base.FMapFormat
         Fiat.Narcissus.Formats.Base.LaxTerminalFormat.
@@ -10,32 +9,38 @@ Require Import
 Section SequenceFormat.
 
   Context {T : Type}. (* Target Type *)
-  Context {cache : Cache}. (* State Type *)
   Context {monoid : Monoid T}. (* Target type is a monoid. *)
+
+  Definition sequence
+             (format1 : Comp T)
+             (format2 : Comp T) :=
+    (p <- format1;
+       q <- format2;
+       ret (mappend p q))%comp.
 
   Definition sequence_Format
              {S : Type}
              (format1 format2 : FormatM S T)
-    := (fun s => compose _ (format1 s) (format2 s))%comp.
+    : FormatM S T := (fun s => sequence (format1 s) (format2 s))%comp.
 
   Definition sequence_Decode
              {S S' : Type}
              (decode1 : DecodeM (S' * T) T)
              (decode2 : S' -> DecodeM S T)
     : DecodeM S T
-    := (fun t env =>
-          match decode1 t env with
-          | Some (s', t', env') => decode2 s' t' env'
+    := (fun t =>
+          match decode1 t with
+          | Some (s', t') => decode2 s' t'
           | None => None
           end).
 
   Definition sequence_Encode
              {S : Type}
              (encode1 encode2 : EncodeM S T)
-    := (fun s env =>
-          `(t1, env') <- encode1 s env ;
-          `(t2, env'') <- encode2 s env';
-          Some (mappend t1 t2, env'')).
+    := (fun s =>
+          t1 <- encode1 s;
+          t2 <- encode2 s;
+          Some (mappend t1 t2)).
 
   Notation "x ++ y" := (sequence_Format x y) : format_scope .
 
@@ -44,39 +49,24 @@ Section SequenceFormat.
         (format1 format2 : FormatM S T)
         (encode1 encode2 : EncodeM S T)
         (encode1_correct : CorrectEncoder format1 encode1)
-        (encode1_consistent : (* If the first format produces *some*
-                                 environment that makes the second format
-                                 (and thus the composite format) non-empty,
-                                 the encoder must also produce an environment
-                                 that makes the second format non-empty. *)
-           forall s env tenv' tenv'',
-             format1 s env ∋ tenv'
-             -> format2 s (snd tenv') ∋ tenv''
-             -> exists tenv3 tenv4,
-                 encode1 s env = Some tenv3
-                 /\ format2 s (snd tenv3) ∋ tenv4)
         (encode2_correct : CorrectEncoder format2 encode2)
     : CorrectEncoder (format1 ++ format2)
                      (sequence_Encode encode1 encode2).
   Proof.
-    unfold CorrectEncoder, sequence_Encode, sequence_Format, compose,
-    DecodeBindOpt, BindOpt in *; intuition; intros.
-    - destruct (encode1 a env) as [ [t1 xxenv] | ] eqn: ? ;
+    unfold CorrectEncoder, sequence_Encode, sequence_Format, sequence,
+    BindOpt in *; intuition; intros.
+    - destruct (encode1 s) as [ t1 | ] eqn: ? ;
         simpl in *; try discriminate.
-      destruct (encode2 a xxenv) as [ [t2 xxxenv] | ] eqn: ? ;
+      destruct (encode2 s) as [ t2 | ] eqn: ? ;
         simpl in *; try discriminate; injections.
       repeat computes_to_econstructor; eauto.
-    -  unfold Bind2 in *; computes_to_inv; destruct v;
-         destruct v0; simpl in *.
-       destruct (encode1 a env) as [ [t1 xxenv] | ] eqn: ? ;
+    - computes_to_inv. simpl in *.
+       destruct (encode1 s) as [ t1 | ] eqn: ? ;
         simpl in *; try discriminate; eauto.
        eapply H2; try eassumption.
-       destruct (encode2 a xxenv) as [ [t2' xxxenv] | ] eqn: ? ;
+       destruct (encode2 s) as [ t2 | ] eqn: ? ;
         simpl in *; try discriminate; injections.
-       specialize (encode1_consistent _ _ _ _ H4 H4');
-         destruct_ex; split_and.
-       rewrite H6 in Heqo; injections; simpl in *.
-       destruct x0; elimtype False; eauto.
+       reflexivity.
   Qed.
 
   Lemma CorrectDecoder_sequence
@@ -86,47 +76,45 @@ Section SequenceFormat.
         (format1 format2 : FormatM S T)
         (decode1 : DecodeM (S' * T) T)
         (decode2 : S' -> DecodeM S T)
-        (format1_overlap : forall s env tenv',
-            format1 s env ∋ tenv' -> exists s',
-              forall t, format1' (s', t) env ∋ (mappend (fst tenv') t, snd tenv') /\ f s s')
-        (format1'_overlap : forall s' t env tenv',
-            format1' (s', t) env ∋ tenv'
+        (format1_overlap : forall s t',
+            format1 s ∋ t' -> exists s',
+              forall t, format1' (s', t) ∋ (mappend t' t) /\ f s s')
+        (format1'_overlap : forall s' t t'',
+            format1' (s', t) ∋ t''
             -> forall s,
               f s s'
-              -> exists t', format1 s env ∋ (t', snd tenv') /\ fst tenv' = mappend t' t)
+              -> exists t', format1 s ∋ t' /\ t'' = mappend t' t)
         (decode1_correct : CorrectDecoder_simpl format1' decode1)
         (decode2_correct : forall (s' : S'), CorrectDecoder_simpl (Restrict_Format (fun s => f s s') format2) (decode2 s'))
     : CorrectDecoder_simpl (format1 ++ format2)
                            (sequence_Decode decode1 decode2).
   Proof.
     unfold CorrectDecoder_simpl, Projection_Format,
-    sequence_Decode, sequence_Format, compose, Compose_Format; split; intros.
-    - unfold Bind2 in H0; computes_to_inv; subst.
-      eapply format1_overlap in H0; destruct_ex; split_and.
-      rewrite @unfold_computes in H0'.
-      destruct v; destruct v0; simpl in *; injections.
+    sequence_Decode, sequence_Format, sequence, Compose_Format; split; intros.
+    - computes_to_inv; subst.
+      eapply format1_overlap in H; destruct_ex; split_and.
+      simpl in *; injections.
+      rewrite unfold_computes in H'.
       destruct decode1_correct as [? _].
       destruct (decode2_correct x) as [? _].
-      destruct (H0 env env' c (x, t0) (mappend t t0)) as (xenv', (decode1_eq, Equiv_xenv));
-        eauto.
-      rewrite decode1_eq; eauto.
-      eapply H3; eauto.
+      specialize (H (x, v0) (mappend v v0)).
+      rewrite H; eauto.
+      apply H2.
       unfold Restrict_Format, Compose_Format; apply unfold_computes.
       setoid_rewrite unfold_computes; eexists; intuition eauto.
-    - destruct (decode1 bin env') as [ [ [s' t'] xenv'']  | ] eqn: ?; try discriminate.
+    - destruct (decode1 t) as [ [s' t'] | ] eqn: ?; try discriminate.
       destruct decode1_correct as [decode1_correct' decode1_correct].
       specialize (decode2_correct s'); destruct decode2_correct as [_ decode2_correct].
       generalize Heqo; intro Heqo'.
       eapply decode1_correct in Heqo; eauto.
-      destruct_ex; split_and.
-      eapply decode2_correct in H0; eauto.
-      destruct_ex; split_and.
-      eexists; intuition eauto.
+      eapply decode2_correct in H; eauto.
       unfold Restrict_Format, Compose_Format, LaxTerminal_Format, sequence_Format,
-        Bind2 in *; computes_to_inv.
-      rewrite @unfold_computes in H1.
-      destruct_ex; split_and; simpl in *; subst.
+      Bind2 in H.
+      rewrite unfold_computes in H. destruct_ex; split_and.
+      rewrite unfold_computes in H1. split_and. subst.
       eapply format1'_overlap in H2; destruct_ex; split_and; subst; eauto.
+      repeat computes_to_econstructor; eauto.
+      rewrite H2. eauto.
   Qed.
 
   Corollary CorrectDecoder_sequence_Projection
@@ -143,17 +131,16 @@ Section SequenceFormat.
   Proof.
     unfold Projection_Format.
     eapply (CorrectDecoder_sequence (fun s s' => f s = s')); eauto; intros;
-      unfold Projection_Format, Compose_Format, sequence_Format, compose, Bind2, LaxTerminal_Format in *.
+      unfold Projection_Format, Compose_Format, sequence_Format, sequence, Bind2, LaxTerminal_Format in *.
     - rewrite @unfold_computes in H.
       destruct_ex; split_and; subst.
       eexists; intros; intuition.
-      destruct tenv'; simpl; computes_to_econstructor.
+      simpl; computes_to_econstructor.
       rewrite unfold_computes; eauto.
       simpl; computes_to_econstructor; eauto.
     - computes_to_inv; subst.
       apply_in_hyp @unfold_computes; destruct_ex; split_and; subst.
       eexists; simpl; intuition eauto.
-      destruct v; apply unfold_computes; eauto.
   Qed.
 
   (*Corollary CorrectDecoder_sequence_Done
